verify/Flip.v
@@ -74,6 +74,19 @@ Qed.
 
 #[export] Hint Resolve flip_multistep : core.
 
+Lemma flip_evstep : forall tm c c',
+  c -[ tm ]->* c' ->
+  flip_conf c -[ flip tm ]->* flip_conf c'.
+Proof. introv H. induction H; eauto. Qed.
+
+Lemma unflip_evstep : forall tm c c',
+  c -[ flip tm ]->* c' ->
+  flip_conf c -[ tm ]->* flip_conf c'.
+Proof.
+  introv H. apply flip_evstep in H.
+  rewrite flip_involutive in H. exact H.
+Qed.
+
 Lemma flip_halting : forall tm c,
   halting tm c -> halting (flip tm) (flip_conf c).
 Proof.
